Plfl/Init.lean
@@ -16,23 +16,15 @@ macro_rules | `(tactic| is_empty) => `(tactic| apply Function.isEmpty (β := Fal
 abbrev Decidable' α := IsEmpty α ⊕' α
 
 namespace Decidable'
-  def toDecidable : Decidable' α → Decidable (Nonempty α) := by
-    intro
-    | .inr a => right; exact ⟨a⟩
-    | .inl na => left; simpa
+  def toDecidable : Decidable' α → Decidable (Nonempty α) := by intro
+  | .inr a => right; exact ⟨a⟩
+  | .inl na => left; simpa
 end Decidable'
 
 instance [Repr α] : Repr (Decidable' α) where
   reprPrec da n := match da with
   | .inr a => ".inr " ++ reprPrec a n
   | .inl _ => ".inl _"
-
-/--
-`Iff'` is like `Iff`, but allows arbitrary sorts.
--/
-abbrev Iff' a b := a → b × b → a
-
-infix:20 " ↔'" => Iff'
 
 theorem congr_arg₃
 (f : α → β → γ → δ) {x x' : α} {y y' : β} {z z' : γ}
